Prove DFT preserves lowered FMP opcodes

venom/passes/dft/proofs/dftStructuralScript.sml
@@ -832,3 +832,147 @@ Proof
      gvs[]) >>
   gvs[dft_invoke_subset_def, dft_invoke_targets_def]
 QED
+
+
+(* ===== Raw FMP opcode preservation ===== *)
+Theorem dft_flip_no_raw[local]:
+  is_flippable inst.inst_opcode /\
+  ~is_raw_fmp_opcode inst.inst_opcode ==>
+  ~is_raw_fmp_opcode (flip_operands inst).inst_opcode
+Proof
+  rpt strip_tac >>
+  Cases_on `inst.inst_operands` >> fs[flip_operands_def] >>
+  Cases_on `t` >> fs[flip_operands_def] >>
+  Cases_on `t'` >> fs[flip_operands_def] >>
+  Cases_on `inst.inst_opcode` >>
+  gvs[is_flippable_def, is_commutative_def, is_comparator_def,
+      flip_comparison_opcode_def, is_raw_fmp_opcode_def]
+QED
+
+Theorem from_block_no_raw[local]:
+  from_block block_insts i /\
+  EVERY (\j. ~is_raw_fmp_opcode j.inst_opcode) block_insts ==>
+  ~is_raw_fmp_opcode i.inst_opcode
+Proof
+  simp[from_block_def, listTheory.EVERY_MEM] >>
+  metis_tac[dft_flip_no_raw]
+QED
+
+Theorem dft_block_no_raw[local]:
+  EVERY (\i. ~is_raw_fmp_opcode i.inst_opcode) bb.bb_instructions ==>
+  EVERY (\i. ~is_raw_fmp_opcode i.inst_opcode)
+        (dft_block order bb).bb_instructions
+Proof
+  simp[listTheory.EVERY_MEM] >> rpt strip_tac >>
+  Cases_on `is_pseudo i.inst_opcode`
+  >- (`MEM i (FILTER (\i. is_pseudo i.inst_opcode)
+                  (dft_block order bb).bb_instructions)` by
+        (simp[listTheory.MEM_FILTER]) >>
+      qpat_x_assum `MEM i (FILTER _ _)` mp_tac >>
+      rewrite_tac[dft_block_phis] >>
+      simp[listTheory.MEM_FILTER] >>
+      metis_tac[]) >>
+  `MEM i (FILTER (\i. ~is_pseudo i.inst_opcode)
+                (dft_block order bb).bb_instructions)` by
+    (simp[listTheory.MEM_FILTER]) >>
+  drule dft_block_from_orig >>
+  simp[from_block_def] >> metis_tac[dft_flip_no_raw]
+QED
+
+Definition dft_blocks_no_raw_def[local]:
+  dft_blocks_no_raw blocks <=>
+    EVERY (\bb. EVERY (\i. ~is_raw_fmp_opcode i.inst_opcode)
+                       bb.bb_instructions) blocks
+End
+
+Theorem dft_blocks_no_raw_fn_insts[local]:
+  dft_blocks_no_raw blocks <=>
+  !inst. MEM inst (fn_insts_blocks blocks) ==>
+         ~is_raw_fmp_opcode inst.inst_opcode
+Proof
+  rewrite_tac[dft_blocks_no_raw_def] >>
+  Induct_on `blocks` >>
+  simp[fn_insts_blocks_def, listTheory.EVERY_MEM,
+       listTheory.MEM_APPEND, DISJ_IMP_THM, FORALL_AND_THM]
+QED
+
+Theorem dft_map_update_no_raw[local]:
+  dft_blocks_no_raw blocks /\ MEM chosen blocks ==>
+  dft_blocks_no_raw
+    (MAP (\b. if b.bb_label = lbl then dft_block order chosen else b) blocks)
+Proof
+  simp[dft_blocks_no_raw_def, listTheory.EVERY_MAP] >>
+  strip_tac >>
+  irule listTheory.EVERY_MONOTONIC >>
+  qexists `\b. EVERY (\i. ~is_raw_fmp_opcode i.inst_opcode)
+                  b.bb_instructions` >> simp[] >>
+  rpt strip_tac >> Cases_on `x.bb_label = lbl` >> simp[] >>
+  irule dft_block_no_raw >>
+  qpat_x_assum `EVERY _ blocks` mp_tac >>
+  simp[listTheory.EVERY_MEM] >> metis_tac[]
+QED
+
+Theorem dft_process_one_no_raw[local]:
+  dft_blocks_no_raw st.dls_blocks ==>
+  dft_blocks_no_raw (FST (dft_process_one cfg lr fn st lbl)).dls_blocks
+Proof
+  strip_tac >> simp[dft_process_one_def] >>
+  Cases_on `lookup_block lbl st.dls_blocks`
+  >- simp[]
+  >> simp[] >> rpt (pairarg_tac >> gvs[]) >>
+  Cases_on `FLOOKUP st.dls_last_order lbl` >> gvs[]
+  >- (Cases_on `x = q` >> gvs[] >>
+      irule dft_map_update_no_raw >> simp[] >>
+      gvs[lookup_block_def] >> metis_tac[dft_FIND_MEM])
+  >> Cases_on `x' = order` >> gvs[] >>
+     irule dft_map_update_no_raw >> simp[] >>
+     gvs[lookup_block_def] >> metis_tac[dft_FIND_MEM]
+QED
+
+Theorem dft_loop_step_no_raw[local]:
+  dft_blocks_no_raw (FST trip).dls_blocks ==>
+  dft_blocks_no_raw (FST (dft_loop_step cfg lr fn trip)).dls_blocks
+Proof
+  Cases_on `trip` >> PairCases_on `r` >>
+  simp[dft_loop_step_def] >>
+  Cases_on `r1` >> simp[] >>
+  Cases_on `r0` >> simp[] >>
+  Cases_on `dft_process_one cfg lr fn q h` >>
+  PairCases_on `r` >> simp[] >>
+  Cases_on `r1` >> simp[] >>
+  Cases_on `r0` >> simp[] >>
+  strip_tac >>
+  `dft_blocks_no_raw
+     (FST (dft_process_one cfg lr fn q h)).dls_blocks` by
+    (irule dft_process_one_no_raw >> simp[]) >>
+  gvs[]
+QED
+
+Theorem dft_funpow_no_raw[local]:
+  !trip. dft_blocks_no_raw (FST trip).dls_blocks ==>
+    dft_blocks_no_raw
+      (FST (FUNPOW (dft_loop_step cfg lr fn) n trip)).dls_blocks
+Proof
+  Induct_on `n`
+  >- simp[] >>
+  gen_tac >> simp[arithmeticTheory.FUNPOW_SUC] >>
+  metis_tac[dft_loop_step_no_raw]
+QED
+
+Theorem dft_fn_no_raw_fmp_ops:
+  no_raw_fmp_ops fn ==> no_raw_fmp_ops (dft_fn fn)
+Proof
+  simp[dft_fn_def, no_raw_fmp_ops_def, fn_insts_def,
+       GSYM dft_blocks_no_raw_fn_insts] >>
+  pairarg_tac >> gvs[] >> strip_tac >>
+  `dft_blocks_no_raw
+     (FST
+       (FUNPOW
+         (dft_loop_step (cfg_analyze fn) (liveness_analyze fn) fn)
+         (LENGTH fn.fn_blocks * LENGTH fn.fn_blocks)
+         (<| dls_blocks := fn.fn_blocks; dls_from_to := FEMPTY;
+              dls_last_order := FEMPTY |>,
+          (cfg_analyze fn).cfg_dfs_post, F))).dls_blocks` by
+    (irule dft_funpow_no_raw >> simp[]) >>
+  gvs[]
+QED
